proof: beginning of fixes for the ERC-20 proof

CoqOfRust/examples/default/examples/ink_contracts/simulations/erc20.v
@@ -2,6 +2,7 @@ Require Import CoqOfRust.CoqOfRust.
 Require CoqOfRust.core.simulations.default.
 Require CoqOfRust.core.simulations.option.
 Require CoqOfRust.examples.default.examples.ink_contracts.simulations.lib.
+Require Import CoqOfRust.lib.simulations.lib.
 Require Import CoqOfRust.simulations.M.
 
 Import simulations.M.Notations.
@@ -9,29 +10,22 @@ Import simulations.M.Notations.
 (** ** Primitives *)
 
 Module Balance.
-  Inductive t : Set :=
-  | Make (balance : Z).
-
-  Global Instance IsToValue : ToValue t := {
-    Φ := Ty.path "erc20::Balance";
-    φ '(Make x) := Value.Integer Integer.U128 x;
-  }.
+  Definition t : Set := u128.t.
 End Balance.
 
 Module Impl_Default_for_Balance.
   Global Instance I : core.simulations.default.Default.Trait Balance.t := {
-    default := Balance.Make 0;
+    default := u128.Make 0;
   }.
 End Impl_Default_for_Balance.
 
 Module AccountId.
   Inductive t : Set :=
-  | Make (account_id : Z).
+  | Make (account_id : u128.t).
 
   Global Instance IsToValue : ToValue t := {
     Φ := Ty.path "erc20::AccountId";
-    φ '(Make x) :=
-      Value.StructTuple "erc20::AccountId" [Value.Integer Integer.U128 x];
+    φ '(Make x) := Value.StructTuple "erc20::AccountId" [φ x];
   }.
 End AccountId.
 
@@ -170,7 +164,7 @@ Definition balance_of_impl
     erc20.Balance.t :=
   match simulations.lib.Mapping.get owner storage.(erc20.Erc20.balances) with
   | Some balance => balance
-  | None => Balance.Make 0
+  | None => u128.Make 0
   end.
 
 Definition balance_of
@@ -190,7 +184,7 @@ Definition allowance_impl
       storage.(erc20.Erc20.allowances)
   with
   | Some allowance => allowance
-  | None => Balance.Make 0
+  | None => u128.Make 0
   end.
 
 Definition allowance
@@ -212,12 +206,11 @@ Definition transfer_from_to
     (value : erc20.Balance.t) :
     MS? State.t string (erc20.Result.t unit) :=
   letS? '(storage, events) := readS? in
-  let 'Balance.Make value := value in
-  let 'Balance.Make from_balance := balance_of_impl storage from in
-  if from_balance <? value then
+  let from_balance := u128.get (balance_of_impl storage from) in
+  if from_balance <? u128.get value then
     returnS? (inr erc20.Error.InsufficientBalance)
   else
-    let new_from_balance := Balance.Make (from_balance - value) in
+    let new_from_balance := u128.Make (from_balance - u128.get value) in
     letS? _ := writeS? (
       storage <| erc20.Erc20.balances :=
         simulations.lib.Mapping.insert from new_from_balance
@@ -226,19 +219,19 @@ Definition transfer_from_to
       events
     ) in
     letS? '(storage, events) := readS? in
-    let 'Balance.Make to_balance := balance_of_impl storage to in
+    let 'u128.Make to_balance := balance_of_impl storage to in
     letS? new_to_balance :=
       return?toS? (
-        Integer.normalize_with_error Integer.U128 (to_balance + value)
+        Integer.normalize_with_error Integer.U128 (to_balance + u128.get value)
       ) in
     let event := erc20.Event.Transfer {|
       erc20.Transfer.from := Some from;
       erc20.Transfer.to := Some to;
-      erc20.Transfer.value := Balance.Make value
+      erc20.Transfer.value := value
     |} in
     letS? _ := writeS? (
       storage <| erc20.Erc20.balances :=
-        simulations.lib.Mapping.insert to (Balance.Make new_to_balance)
+        simulations.lib.Mapping.insert to (u128.Make new_to_balance)
           storage.(erc20.Erc20.balances)
       |>,
       event :: events
@@ -281,16 +274,16 @@ Definition transfer_from
     MS? State.t string (erc20.Result.t unit) :=
   let caller := Env.caller env in
   letS? '(storage, events) := readS? in
-  let 'Balance.Make value := value in
-  let 'Balance.Make allowance := allowance_impl storage from caller in
+  let 'u128.Make value := value in
+  let 'u128.Make allowance := allowance_impl storage from caller in
   if allowance <? value then
     returnS? (inr erc20.Error.InsufficientAllowance)
   else
-    letS? result_from_to := transfer_from_to from to (Balance.Make value) in
+    letS? result_from_to := transfer_from_to from to (u128.Make value) in
     match result_from_to with
     | inr _ => returnS? (result_from_to)
     | inl _ =>
-      let new_allowance := Balance.Make (allowance - value) in
+      let new_allowance := u128.Make (allowance - value) in
       letS? '(storage, events) := readS? in
       letS? _ := writeS? (
         storage <| erc20.Erc20.allowances :=
